Types/AbstractBool.v
@@ -5,13 +5,11 @@ Require Import Coq.Bool.Bool.
 Inductive abstr_bool : Type :=
   | ab_true   : abstr_bool
   | ab_false  : abstr_bool
-  | ab_top    : abstr_bool
-  | ab_bottom : abstr_bool.
+  | ab_top    : abstr_bool.
 
 (** * Correspondence with bool *)
 
 Inductive ab_le : abstr_bool -> abstr_bool -> Prop :=
-  | ab_le_bottom : forall ab, ab_le ab_bottom ab
   | ab_le_top : forall ab, ab_le ab ab_top
   | ab_le_refl : forall ab, ab_le ab ab.
 
@@ -26,7 +24,6 @@ Definition gamma_bool (ab: abstr_bool) (b : bool) : Prop :=
   | ab_true   => Is_true b
   | ab_false  => ~Is_true b
   | ab_top    => True
-  | ab_bottom => False
   end.
 
 Definition extract_bool (b: bool) : abstr_bool :=
@@ -35,29 +32,20 @@ Definition extract_bool (b: bool) : abstr_bool :=
   | false => ab_false
   end.
 
-
-
-
 (** * Operations *)
 
 (** ** And *)
 
 Definition and_ab (b1 b2 : abstr_bool) : abstr_bool :=
   match b1 with
-  | ab_bottom => ab_bottom
   | ab_true   => b2
   | ab_top    => match b2 with
-                 | ab_bottom => ab_bottom
                  | ab_false  => ab_false
                  | _         => ab_top
                  end
-  | ab_false  => match b2 with
-                 | ab_bottom => ab_bottom
-                 | _ => ab_false
-                 end
+  | ab_false  => ab_false
   end.
 
-Example and_ab1 : and_ab ab_bottom ab_top = ab_bottom. reflexivity. Qed.
 Example and_ab2 : and_ab ab_true ab_true = ab_true. reflexivity. Qed.
 Example and_ab3 : and_ab ab_true ab_false = ab_false. reflexivity. Qed.
 Example and_ab4 : and_ab ab_top  ab_true = ab_top. reflexivity. Qed.
@@ -79,17 +67,12 @@ Proof. destruct ab1, b1, ab2, b2; simpl; tauto. Qed.
 
 Definition or_ab (b1 b2 : abstr_bool) : abstr_bool :=
   match b1 with
-  | ab_bottom => ab_bottom
   | ab_false  => b2
   | ab_top    => match b2 with
-                 | ab_bottom => ab_bottom
                  | ab_true   => ab_true
                  | _         => ab_top
                  end
-  | ab_true   => match b2 with
-                 | ab_bottom => ab_bottom
-                 | _         => ab_true
-                 end
+  | ab_true   => ab_true
   end.
 
 Lemma or_ab_comm : forall b1 b2, or_ab b1 b2 = or_ab b2 b1.
@@ -127,7 +110,6 @@ Proof. destruct ab, b; simpl; tauto. Qed.
 (** ** Join *)
 Definition ab_join (ab1 ab2 : abstr_bool) : abstr_bool :=
   match ab1, ab2 with
-  | ab_bottom, b | b, ab_bottom => b
   | ab_top, _ | _, ab_top => ab_top
   | ab_true, ab_true => ab_true
   | ab_false, ab_false => ab_false
@@ -152,25 +134,3 @@ Proof.
   intros. destruct ab; auto.
 Qed.
 
-(** ** Meet *)
-Definition ab_meet (ab1 ab2 : abstr_bool) : abstr_bool :=
-  match ab1, ab2 with
-  | ab_bottom, _ | _, ab_bottom => ab_bottom
-  | ab_top, b | b, ab_top => b
-  | ab_true, ab_true => ab_true
-  | ab_false, ab_false => ab_false
-  | ab_true, ab_false | ab_false, ab_true => ab_bottom
-  end.
-
-
-Lemma ab_meet_assoc : forall (ab1 ab2 : abstr_bool),
-  ab_meet ab1 ab2 = ab_meet ab2 ab1.
-Proof. 
-  intros. destruct ab1, ab2; auto.
-Qed.
-
-Lemma ab_meet_idem : forall ab,
-  ab_meet ab ab = ab.
-Proof. 
-  intros. destruct ab; auto. 
-Qed.
