Classes/Monad/MonadParallel.v
@@ -1,0 +1,6 @@
+Require Import Classes.Monad.
+
+Class MonadParallel (M : Type → Type) `{Monad M} :=
+{
+  bindM2 : ∀ {A B C}, M A → M B → (A → B → M C) → M C;
+}.
